{
 "cells": [
  {
   "cell_type": "markdown",
   "metadata": {},
   "source": [
    "## Theorem 4.1: Composition of two linear maps is also a linear map\n",
    "\n",
    "Let $U, V, W$ be vector spaces over a field $K$. Let\n",
    "\n",
    "$$\n",
    "\\begin{aligned}\n",
    "F: U \\to V &&\\text{and}&& G: V \\to W\n",
    "\\end{aligned}\n",
    "$$\n",
    "\n",
    "be linear maps. Then the composition map $G \\circ F$ is also a linear map.\n",
    "\n",
    "### Proof\n",
    "\n",
    "$G \\circ F$ is a map from $U$ to $W$.\n",
    "\n",
    "#### LM 1\n",
    "\n",
    "For any $u, v \\in U$, since $F, G$ are linear maps, we have\n",
    "\n",
    "$$\n",
    "(G \\circ F)(u + v) = G(F(u + v)) = G(F(u) + F(v)) = G(F(u)) + G(F(v)) = (G \\circ F)(u) + (G \\circ F)(v)\n",
    "$$\n",
    "\n",
    "#### LM 2\n",
    "\n",
    "For any $u \\in U$, for any $c \\in K$, since $F, G$ are linear maps, we have\n",
    "\n",
    "$$\n",
    "(G \\circ F)(c u) = G(F(c u)) = G(c F(u)) = c G(F(u)) = c ((G \\circ F)(u))\n",
    "$$\n",
    "\n",
    "Hence $(G \\circ F)$ is a linear map. Q.E.D."
   ]
  },
  {
   "cell_type": "markdown",
   "metadata": {},
   "source": [
    "## Theorem 4.2. Algebraic rules for linear map compositions\n",
    "\n",
    "Let $U, V, W$ be vector spaces over a field $K$. Let\n",
    "\n",
    "$$\n",
    "F: U \\to V\n",
    "$$\n",
    "\n",
    "be a linear mapping, and let $G, H$ be two linear mappings of $V$ into $W$.\n",
    "\n",
    "Then\n",
    "\n",
    "$$\n",
    "(G + H) \\circ F = G \\circ F + H \\circ F\n",
    "$$\n",
    "\n",
    "If $c$ is a number, then\n",
    "\n",
    "$$\n",
    "(c G) \\circ F = c (G \\circ F)\n",
    "$$\n",
    "\n",
    "If $T: U \\to V$ is a linear mapping from $U$ into $V$, then\n",
    "\n",
    "$$\n",
    "G \\circ (F + T) = G \\circ F + G \\circ T\n",
    "$$\n",
    "\n",
    "### Proof\n",
    "\n",
    "#### Proof: $(G + H) \\circ F = G \\circ F + H \\circ F$\n",
    " \n",
    "For any $u \\in U$, we have\n",
    "\n",
    "$$\n",
    "((G + H) \\circ F)(u) = ((G + H)(F(u)))\n",
    "$$\n",
    "\n",
    "By the [definition](3_2_linear_mappings.ipynb#Sum) of sums of linear mappings, we have\n",
    "\n",
    "$$\n",
    "((G + H)(F(u))) = G(F(u)) + H(F(u)) = (G \\circ F)(u) + (H \\circ F)(u)\n",
    "$$\n",
    "\n",
    "\n",
    "Thus \n",
    "\n",
    "$$\n",
    "(G + H) \\circ F = G \\circ F + H \\circ F\n",
    "$$\n",
    "\n",
    "#### Proof: $(c G) \\circ F = c (G \\circ F)$\n",
    "\n",
    "For any $u \\in U$, we have\n",
    "\n",
    "$$\n",
    "((c G) \\circ F)(u) = (c G)(F(u))\n",
    "$$\n",
    "\n",
    "By the [definition](3_2_linear_mappings.ipynb#Scalar-multiplication) of scalar products of linear mappings, we have\n",
    "\n",
    "$$\n",
    "(c G)(F(u)) = c (G(F(u))) = c ((G \\circ F)(u))\n",
    "$$\n",
    "\n",
    "Thus\n",
    "\n",
    "$$\n",
    "(c G) \\circ F) = c (G \\circ F)\n",
    "$$\n",
    "\n",
    "#### Proof: $G \\circ (F + T) = G \\circ F + G \\circ T$\n",
    "\n",
    "For any $u \\in U$, we have\n",
    "\n",
    "$$\n",
    "(G \\circ (F + T))(u) = G((F + T)(u)) = G(F(u) + T(u))\n",
    "$$\n",
    "\n",
    "And since $G$ is a linear map, we have\n",
    "\n",
    "$$\n",
    "G(F(u) + T(u)) = G(F(u)) + G(T(u)) = (G \\circ F)(u) + (G \\circ T)(u)\n",
    "$$\n",
    "\n",
    "Hence\n",
    "\n",
    "$$\n",
    "G \\circ (F + T) = G \\circ F + G \\circ T\n",
    "$$\n",
    "\n",
    "Q.E.D."
   ]
  },
  {
   "cell_type": "code",
   "execution_count": null,
   "metadata": {},
   "outputs": [],
   "source": []
  }
 ],
 "metadata": {
  "kernelspec": {
   "display_name": "Python 3",
   "language": "python",
   "name": "python3"
  },
  "language_info": {
   "codemirror_mode": {
    "name": "ipython",
    "version": 3
   },
   "file_extension": ".py",
   "mimetype": "text/x-python",
   "name": "python",
   "nbconvert_exporter": "python",
   "pygments_lexer": "ipython3",
   "version": "3.7.0"
  }
 },
 "nbformat": 4,
 "nbformat_minor": 2
}
