{
 "cells": [
  {
   "cell_type": "markdown",
   "metadata": {},
   "source": [
    "## 1. Let $L: R^2 \\to R^2$ be a linear map such that $L \\neq \\mathit{0}$ but $L^2 = L \\circ L = \\mathit{0}$. Show that there exists a basis $\\{A, B\\}$ of $R^2$ such that\n",
    "\n",
    "$$\n",
    "\\begin{aligned}\n",
    "L(A) = B && \\text{and} && L(B) = \\mathit{0}\n",
    "\\end{aligned}\n",
    "$$\n",
    "\n",
    "### Proof\n",
    "\n",
    "Since $L \\neq \\mathit{0}$, we let $A$ be any vector in $R^2$ such that $A \\neq \\mathit{0}$ and $L(A) \\neq \\mathit{0}$. Let $B = L(A)$. We also have $B \\neq 0$.\n",
    "\n",
    "Then we have\n",
    "\n",
    "$$\n",
    "L(B) = L(L(A)) = L^2(A) = \\mathit{0}(A) = \\mathit{0}\n",
    "$$\n",
    "\n",
    "Now we contend $\\{A, B\\}$ is a basis of $R^2$.\n",
    "\n",
    "Let $\\alpha, \\beta$ be numbers in $R$ such that\n",
    "\n",
    "$$\n",
    "\\alpha A + \\beta B = \\mathit{0}\n",
    "$$\n",
    "\n",
    "Then we have\n",
    "\n",
    "$$\n",
    "L(\\alpha A + \\beta B) = L(\\mathit{0})\n",
    "$$\n",
    "\n",
    "And since [the linear mapping of zero vector is also a zero vector](../3_2_linear_mappings.ipynb#Linear-mapping-at-zero-vector-$\\mathit{0}$), we have\n",
    "\n",
    "$$\n",
    "L(\\alpha A + \\beta B) = \\mathit{0}\n",
    "$$\n",
    "\n",
    "Hence\n",
    "\n",
    "$$\n",
    "\\alpha L(A) + \\beta L(B) = \\alpha L(A) + \\beta L^2(A) = \\alpha L(A) = \\mathit{0}\n",
    "$$\n",
    "\n",
    "Thus\n",
    "\n",
    "$$\n",
    "\\alpha L(A) = \\alpha B = \\mathit{0}\n",
    "$$\n",
    "\n",
    "And since $B \\neq \\mathit{0}$, we have\n",
    "\n",
    "$$\n",
    "\\alpha = 0\n",
    "$$\n",
    "\n",
    "Now we know the only $\\alpha, \\beta$ for\n",
    "\n",
    "$$\n",
    "\\alpha A + \\beta B = \\mathit{0}\n",
    "$$\n",
    "\n",
    "to hold is $\\alpha = 0, \\beta = 0$.\n",
    "\n",
    "Hence $A, B$ are linear independent.\n",
    "\n",
    "And since $\\dim R^2 = 2$, by [theorem 3.3 in chapter 1](../../1_vector_spaces/1_vector_spaces.ipynb#Theorem-3.3.) we know $\\{A, B\\}$ is a basis of $R^2$.\n",
    "\n",
    "Q.E.D."
   ]
  },
  {
   "cell_type": "markdown",
   "metadata": {},
   "source": [
    "## 2.  Let $\\dim V > \\dim W$. Let $L: V \\to W$ be a linear map. Show that the kernel of $L$ is not $\\{\\mathit{0}\\}$.\n",
    "\n",
    "### Proof\n",
    "\n",
    "From [theorem 3.3](../3_3_kernel_and_image_of_a_linear_map.ipynb#Theorem-3.2:-Kernel,-image,-and-dimensions), we know\n",
    "\n",
    "$$\n",
    "\\dim V = \\dim \\operatorname{Ker} L + \\dim \\operatorname{Im} L\n",
    "$$\n",
    "\n",
    "And since $\\operatorname{Im} L$ [is a subspace of](../3_3_kernel_and_image_of_a_linear_map.ipynb#Image-of-a-linear-map-as-a-subspace) $W$, by [theorem 3.1 in chapter 1](../../1_vector_spaces.ipynb#Theorem-3.7.) we have\n",
    "\n",
    "$$\n",
    "\\dim \\operatorname{Im} L \\leq \\dim W\n",
    "$$\n",
    "\n",
    "And since $\\dim V > \\dim W$, we know $\\dim V - \\dim W > 0$. Hence\n",
    "\n",
    "$$\n",
    "\\dim \\operatorname{Ker} L = \\dim V - \\dim \\operatorname{Im} L \\geq \\dim V - \\dim W > 0\n",
    "$$\n",
    "\n",
    "Hence\n",
    "\n",
    "$$\n",
    "\\dim \\operatorname{Ker} L > 0\n",
    "$$\n",
    "\n",
    "Hence\n",
    "\n",
    "$$\n",
    "\\operatorname{Ker} L \\neq \\{0\\}\n",
    "$$\n",
    "\n",
    "Q.E.D."
   ]
  },
  {
   "cell_type": "markdown",
   "metadata": {},
   "source": [
    "## 3.  Finish the proof of Theorem 4.3.\n",
    "\n",
    "[Done](../3_4_composition_and_inverse_of_linear_mappings.ipynb#Theorem-4.3.)."
   ]
  },
  {
   "cell_type": "markdown",
   "metadata": {},
   "source": [
    "## 4. Let $\\dim V = \\dim W$. Let $L:V \\to W$ be a linear map whose kernel is $\\{\\mathit{0}\\}$. Show that $L$ has an inverse linear map.\n",
    "\n",
    "\n",
    "### Proof\n",
    "\n",
    "Since $L$ is a linear map, $\\dim V = \\dim W$, and $\\operatorname{Ker} L = \\{\\mathit{0}\\}$ by [theorem 3.3](../3_3_kernel_and_image_of_a_linear_map.ipynb#Theorem-3.3:-Kernel,-dimensions,-and-bijectivity), we have $L$ is bijective. Hence $L$ is surjective.\n",
    "\n",
    "And by [corollary 3.4](../3_linear_mappings/3_4_composition_and_inverse_of_linear_mappings.ipynb#Corollary-4.4.), we have $L$ having an inverse linear map."
   ]
  },
  {
   "cell_type": "markdown",
   "metadata": {},
   "source": [
    "## 5. Let $F, G$ be invertible linear maps of a vector space $V$ onto itself. Show that\n",
    "\n",
    "$$\n",
    "(F \\circ G)^{-1} = G^{-1} \\circ F^{-1}\n",
    "$$\n",
    "\n",
    "### Proof\n",
    "\n",
    "#### Lemma 5.1\n",
    "\n",
    "Linear mapping composition is associative. A.k.a\n",
    "\n",
    "Let $F, G, H$ be invertible linear maps of a vector space $V$ onto itself. We have\n",
    "\n",
    "$$\n",
    "(F \\circ G) \\circ H = F \\circ (G \\circ H)\n",
    "$$\n",
    "\n",
    "##### Proof: Lemma 5.1\n",
    "\n",
    "Let $v$ be any element of $V$. We have\n",
    "\n",
    "$$\n",
    "((F \\circ G) \\circ H)(v) = (F \\circ G)(H(v)) = F(G(H(v))) = F((G \\circ H)(v)) = (F \\circ (G \\circ H))(v)\n",
    "$$\n",
    "\n",
    "Hence\n",
    "\n",
    "$$\n",
    "(F \\circ G) \\circ H = F \\circ (G \\circ H)\n",
    "$$\n",
    "\n",
    "#### Proof: $(F \\circ G)^{-1} = G^{-1} \\circ F^{-1}$\n",
    "\n",
    "From [Lemma 5.1](#Proof:-Lemma-5.1), we have\n",
    "\n",
    "$$\n",
    "\\begin{aligned}\n",
    "(F \\circ G) \\circ (G^{-1} \\circ F^{-1}) &= ((F \\circ G) \\circ G^{-1}) \\circ F^{-1} \\\\\n",
    "&= (F \\circ (G \\circ G^{-1})) \\circ F^{-1} \\\\\n",
    "&= (F \\circ I) \\circ F^{-1} \\\\\n",
    "&= F \\circ F^{-1} \\\\\n",
    "&= I\n",
    "\\end{aligned}\n",
    "$$\n",
    "\n",
    "and\n",
    "\n",
    "$$\n",
    "\\begin{aligned}\n",
    "(G^{-1} \\circ F^{-1}) \\circ (F \\circ G) &= ((G^{-1} \\circ F^{-1}) \\circ F) \\circ G \\\\\n",
    "&= (G^{-1} \\circ (F^{-1} \\circ F)) \\circ G \\\\\n",
    "&= (G^{-1} \\circ I) \\circ G \\\\\n",
    "&= G^{-1} \\circ G \\\\\n",
    "&= I\n",
    "\\end{aligned}\n",
    "$$\n",
    "\n",
    "Hence $G^{-1} \\circ F^{-1}$ is the inverse of $F \\circ G$. Q.E.D."
   ]
  },
  {
   "cell_type": "markdown",
   "metadata": {},
   "source": [
    "## 6. \n",
    "\n",
    "Let $L: R^2 \\circ R^2$ be the linear map defined by\n",
    "\n",
    "$$\n",
    "L(x, y) = (x + y, x - y)\n",
    "$$\n",
    "\n",
    "Show that $L$ is invertible.\n",
    "\n",
    "### Proof\n",
    "\n",
    "#### Proof by concrete example\n",
    "\n",
    "If such an inverse exist, the composition of $L$ and the inverse should return $(x, y)$. And in order to find the relationship between $(x, y)$ and $(x + y, x - y)$ we observe that\n",
    "\n",
    "$$\n",
    "\\begin{cases}\n",
    "x &= \\frac{(x + y) + (x - y)}{2} \\\\\n",
    "y &= \\frac{(x + y) - (x - y)}{2}\n",
    "\\end{cases}\n",
    "$$\n",
    "\n",
    "Let $L^\\prime: R^2 \\circ R^2$ be map defined by\n",
    "\n",
    "$$\n",
    "L^\\prime(x, y) = (\\frac{x + y}{2}, \\frac{x - y}{2})\n",
    "$$\n",
    "\n",
    "It's obvious that $L^{\\prime}$ is a linear map.\n",
    "\n",
    "Then we have\n",
    "\n",
    "$$\n",
    "(L \\circ L^\\prime)(x, y) = L(L^\\prime(x, y)) = L(\\frac{x + y}{2}, \\frac{x - y}{2}) = (\\frac{x + y}{2} + \\frac{x - y}{2}, \\frac{x + y}{2} -\\frac{x - y}{2}) = (x, y)\n",
    "$$\n",
    "\n",
    "$$\n",
    "(L^\\prime \\circ L)(x, y) = L^\\prime(L(x, y)) = L^\\prime(x + y, x - y) = (\\frac{(x + y) + (x - y)}{2}, \\frac{(x + y) - (x - y)}{2}) = (x, y)\n",
    "$$\n",
    "\n",
    "Hence\n",
    "\n",
    "$$\n",
    "L \\circ L^\\prime = L^\\prime \\circ L = I\n",
    "$$\n",
    "\n",
    "Hence $L$ is invertible. Q.E.D.\n",
    "\n",
    "#### Proof by abstract theorems\n",
    "\n",
    "I guess we don't always have the fortune to easily find a good candidate of the inverse function. So let's try to follow a more abstract approach here.\n",
    "\n",
    "##### Proof: $\\operatorname{Ker} L = \\{\\mathit{0}\\}$\n",
    "\n",
    "We contend $\\operatorname{Ker} L = \\{\\mathit{0}\\}$.\n",
    "\n",
    "Let $(x^\\prime, y^\\prime) \\in R^2$ such that \n",
    "\n",
    "$$\n",
    "L(x^\\prime, y^\\prime) = (x^\\prime + y^\\prime, x^\\prime - y^\\prime) = (0, 0)\n",
    "$$\n",
    "\n",
    "Then we have\n",
    "\n",
    "$$\n",
    "\\begin{cases}\n",
    "x^\\prime + y^\\prime &= 0 \\\\\n",
    "x^\\prime - y^\\prime &= 0 \\\\\n",
    "\\end{cases}\n",
    "$$\n",
    "\n",
    "Then we have\n",
    "\n",
    "$$\n",
    "(x^\\prime, y^\\prime) = (0, 0)\n",
    "$$\n",
    "\n",
    "Hence $\\operatorname{Ker} L= \\{\\mathit{0}\\}$.\n",
    "\n",
    "##### Proof: $\\dim \\operatorname{Im} L = \\dim R^2$\n",
    "\n",
    "Since $\\operatorname{Ker} L = \\{\\mathit{0}\\}$, we know $\\dim \\operatorname{Ker} L = 0$. By [theorem 3.3](../3_3_kernel_and_image_of_a_linear_map.ipynb#Theorem-3.2:-Kernel,-image,-and-dimensions), we have\n",
    "\n",
    "\n",
    "Hence\n",
    "$$\n",
    "\\dim R^2 - \\dim \\operatorname{Im} L = \\dim \\operatorname{Ker} L = 0\n",
    "$$\n",
    "\n",
    "Thus\n",
    "\n",
    "$$\n",
    "\\dim R^2 = \\dim \\operatorname{Im} L\n",
    "$$\n",
    "\n",
    "Since $L$ is a linear map from $R^2$ into $R^2$, and $\\dim R^2 = \\dim \\operatorname{Im} L$, and $\\operatorname{Ker} L= \\{\\mathit{0}\\}$, by the conclusion of [exercise 4](#4.-Let-$\\dim-V-=-\\dim-W$.-Let-$L:V-\\to-W$-be-a-linear-map-whose-kernel-is-$\\{\\mathit{0}\\}$.-Show-that-$L$-has-an-inverse-linear-map.), we know $L$ is invertible. Q.E.D."
   ]
  },
  {
   "cell_type": "markdown",
   "metadata": {},
   "source": [
    "## 7. \n",
    "\n",
    "Let $L: R^2 \\to R^2$ be the linear map defined by\n",
    "\n",
    "$$\n",
    "L(x, y) = (2 x + y, 3 x - 5 y)\n",
    "$$\n",
    "\n",
    "Show that $L$ is invertible.\n",
    "\n",
    "### Proof\n",
    "\n",
    "This concrete example is boring. Let's generalize.\n",
    "\n",
    "#### Generalization\n",
    "\n",
    "Let $L: R^2 \\to R^2$ be the linear map defined by\n",
    "\n",
    "$$\n",
    "L(x, y) = (a x + b y, c x + d y)\n",
    "$$\n",
    "\n",
    "for any $a, b, c, d \\in R$ where $(a, c), (b, d)$ are linearly independent. Show that $L$ is invertible.\n",
    "\n",
    "##### Proof: Generalization\n",
    "\n",
    "##### Proof: $\\operatorname{Ker} L = \\{\\mathit{0}\\}$\n",
    "\n",
    "Let $(x^\\prime, y^\\prime)$ be any element in $\\operatorname{Ker} L$. Thus\n",
    "\n",
    "$$\n",
    "L(x^\\prime, y^\\prime) = (a x^\\prime + b y^\\prime, c x^\\prime + d y^\\prime) = \\mathit{0} = (0, 0)\n",
    "$$\n",
    "\n",
    "Thus\n",
    "\n",
    "$$\n",
    "\\begin{cases}\n",
    "a x^\\prime + b y^\\prime &= 0 \\\\\n",
    "c x^\\prime + d y^\\prime &= 0\n",
    "\\end{cases}\n",
    "$$\n",
    "\n",
    "We can write the above system linear equations as\n",
    "\n",
    "$$\n",
    "x^\\prime \\begin{pmatrix}a \\\\ c \\end{pmatrix} + y^\\prime \\begin{pmatrix} b \\\\ d \\end{pmatrix} = \\begin{pmatrix} 0 \\\\ 0\\end{pmatrix}\n",
    "$$\n",
    "\n",
    "Since $(a, c), (b, d)$ are linearly independent, by [theorem 2.2 in chapter 2](../../2_matrices/2_2_linear_equations.ipynb#Theorem-2.2.), know the above system of linear equation has a unique solution.\n",
    "\n",
    "And since $(0, 0)$ is a solution for the above system of linear equations, then we know $x^\\prime = 0, y^\\prime = 0$ is the only solution for above.\n",
    "\n",
    "Hence\n",
    "\n",
    "$$\n",
    "\\operatorname{Ker} L = \\{\\mathit{0}\\}\n",
    "$$\n",
    "\n",
    "##### Proof: $\\dim \\operatorname{Im} L = \\dim R^2$\n",
    "\n",
    "Since $\\operatorname{Ker} L = \\{\\mathit{0}\\}$, we know $\\dim \\operatorname{Ker} L = 0$. By [theorem 3.3](../3_3_kernel_and_image_of_a_linear_map.ipynb#Theorem-3.2:-Kernel,-image,-and-dimensions), we have\n",
    "\n",
    "\n",
    "Hence\n",
    "$$\n",
    "\\dim R^2 - \\dim \\operatorname{Im} L = \\dim \\operatorname{Ker} L = 0\n",
    "$$\n",
    "\n",
    "Thus\n",
    "\n",
    "$$\n",
    "\\dim R^2 = \\dim \\operatorname{Im} L\n",
    "$$\n",
    "\n",
    "Since $L$ is a linear map from $R^2$ into $R^2$, and $\\dim R^2 = \\dim \\operatorname{Im} L$, and $\\operatorname{Ker} L= \\{\\mathit{0}\\}$, by the conclusion of [exercise 4](#4.-Let-$\\dim-V-=-\\dim-W$.-Let-$L:V-\\to-W$-be-a-linear-map-whose-kernel-is-$\\{\\mathit{0}\\}$.-Show-that-$L$-has-an-inverse-linear-map.), we know $L$ is invertible. Q.E.D.\n",
    "\n",
    "##### Proof:  $L(x, y) = (2 x + y, 3 x - 5 y)$  is invertible\n",
    "\n",
    "Since $(2, 3), (1, -5)$ are linearly independent, we can apply the generalized lemma above. Hence $L(x, y) = (2 x + y, 3 x - 5 y)$  is invertible. Q.E.D."
   ]
  },
  {
   "cell_type": "markdown",
   "metadata": {},
   "source": [
    "## 8. Let $L: R^3 \\to R^3$ be the linear maps as indicated. Show that $L$ is invertible in each case.\n",
    "\n",
    "### (a) $L(x, y, z)=(x - y,x + z,x + y + 2z)$\n",
    "\n",
    "### (b) $L(x, y, z) = (2x - y + z, x + y, 3x + y + z)$\n",
    "\n",
    "We can generalize like in exercise 7. Skip."
   ]
  },
  {
   "cell_type": "markdown",
   "metadata": {},
   "source": [
    "## 9.\n",
    "\n",
    "### (a) Let $L:V \\to V$ be a linear mapping such that $L^2 = \\mathit{0}$ .Show that $I - L$ is invertible. ($I$ is the identity mapping on $V$.)\n",
    "\n",
    "#### Proof\n",
    "\n",
    "By theorem [3.4](../3_4_composition_and_inverse_of_linear_mappings.ipynb#Theorem-4.2.-Algebraic-rules-for-linear-map-compositions), we have\n",
    "\n",
    "$$\n",
    "\\begin{aligned}\n",
    "(I - L) \\circ (I + L) &= (I - L) \\circ I + (I - L) \\circ L \\\\\n",
    "&= (I - L) + (I \\circ L - L^2) \\\\\n",
    "&= (I - L) + (L - \\mathit{0}) \\\\\n",
    "&= (I - L) + L \\\\\n",
    "&= I\n",
    "\\end{aligned}\n",
    "$$\n",
    "\n",
    "and\n",
    "\n",
    "$$\n",
    "\\begin{aligned}\n",
    "(I + L) \\circ (I - L) &= (I + L) \\circ I - (I + L) \\circ L \\\\\n",
    "&= (I + L) - (I \\circ L + L^2) \\\\\n",
    "&= (I + L) - (L + \\mathit{0}) \\\\\n",
    "&= I\n",
    "\\end{aligned}\n",
    "$$\n",
    "\n",
    "Hence $I - L$ is invertible as its inverse is $I + L$.\n",
    "\n",
    "Q.E.D."
   ]
  },
  {
   "cell_type": "markdown",
   "metadata": {},
   "source": [
    "### (b) Let $L:V \\to V$ be a linear map such that $L^2 + 2L + I =\\mathit{0}$. Show that $L$ is invertible.\n",
    "\n",
    "#### Proof\n",
    "\n",
    "##### Lemma: If a linear map $F: V \\to U$ is invertible, then $- F$ is also invertible\n",
    "\n",
    "Prof:\n",
    "\n",
    "Since $F$ is a linear map, theorem [3.4](../3_4_composition_and_inverse_of_linear_mappings.ipynb#Theorem-4.2.-Algebraic-rules-for-linear-map-compositions), we have\n",
    "\n",
    "$$\n",
    "(- F) \\circ (- F^{-1}) = ((-1) F) \\circ (- F^{-1}) = - (F \\circ ((-1) F^{-1})) = - (-1) (F \\circ F^{-1}) = I\n",
    "$$\n",
    "\n",
    "and\n",
    "\n",
    "$$\n",
    "(- F^{-1}) \\circ (- F) = ((-1) F^{-1}) \\circ (- F) = - (F^{-1} \\circ ((-1) F)) = - (-1) (F^{-1} \\circ F) = I\n",
    "$$\n",
    "\n",
    "##### Proof by applying the lemma\n",
    "\n",
    "By theorem [3.4](../3_4_composition_and_inverse_of_linear_mappings.ipynb#Theorem-4.2.-Algebraic-rules-for-linear-map-compositions), we have\n",
    "\n",
    "$$\n",
    "L^2 + 2L + I = L^2 + 2 L + I^2 = (L + I) \\circ (L + I) = (L + I)^2 = \\mathit{0}\n",
    "$$\n",
    "\n",
    "Let $L^\\prime = L + I$. Then we have $L^\\prime$ is also a linear map and $L^\\prime = \\mathit{0}$.\n",
    "\n",
    "By the conclusion of **(a)**, we know $I - L^\\prime$ is invertible and its inverse is $I + L^\\prime$.\n",
    "\n",
    "Since $L^\\prime = L + I$, we have $- L = I - L^\\prime$. \n",
    "\n",
    "Hence $- L$ is invertible.\n",
    "\n",
    "By the [lemma above](#Lemma:-If-a-linear-map-$F:-V-\\to-U$-is-invertible,-then-$--F$-is-also-invertible), we know $L = - (- L)$ is also invertible. Q.E.D."
   ]
  },
  {
   "cell_type": "markdown",
   "metadata": {},
   "source": [
    "### (c) Let $L:V \\to V$be a linear map such that $L^3= \\mathit{0}$. Show that $I - L$ is invertible.\n"
   ]
  },
  {
   "cell_type": "markdown",
   "metadata": {},
   "source": [
    "## 10.\n",
    "\n",
    "Let $V$ be a vector space. Let $P:V \\to V$ be a linear map such that $P^2 = P$. Show that\n",
    "\n",
    "$$\n",
    "\\begin{aligned}\n",
    "V = \\operatorname{Ker} P + \\operatorname{Im} P && \\text{and} && \\operatorname{Ker} P \\cap \\operatorname{Im} P = \\{\\mathit{0}\\}\n",
    "\\end{aligned}\n",
    "$$\n",
    "\n",
    "in other words, $V$ is the direct sum of $\\operatorname{Ker} P$ and $\\operatorname{Im} P$. \\[Hint: To show $V$ is the sum, write an element of $V$ in the form $v = v - P v + P v$.\\]\n",
    "\n",
    "**Note**: $P$ is called a [projection](https://en.wikipedia.org/wiki/Projection_(linear_algebra)) if $P^2 = P$.\n",
    "\n",
    "### Proof\n",
    "\n",
    "For any $v \\in V$, since $P$ is a linear map from $V$ into $V$, we can write $v$ as\n",
    "\n",
    "$$\n",
    "v = v - P v + P v\n",
    "$$\n",
    "\n",
    "#### Proof: $\\{v^\\prime \\in V | [\\exists v \\in V] v^\\prime = v - P v\\} = \\operatorname{Ker} P$\n",
    "\n",
    "Let $V^\\prime = \\{v^\\prime \\in V | [\\exists v \\in V] v^\\prime = v - P v\\}$.\n",
    "\n",
    "We first contend $V^\\prime = \\operatorname{Ker} P$ by showing $V^\\prime \\subseteq \\operatorname{Ker} P$ and $\\operatorname{Ker} P \\subseteq V^\\prime$.\n",
    "\n",
    "For any $v^\\prime \\in V^\\prime$, there exists some $v \\in V$ such that\n",
    "\n",
    "$$\n",
    "P v^\\prime = P(v - P v) = P v - P^2 v = P v - P v = \\mathit{0}\n",
    "$$\n",
    "\n",
    "Hence $V^\\prime \\subseteq \\operatorname{Ker} P$.\n",
    "\n",
    "Let $v^\\prime \\in \\operatorname{Ker} P$. Then we have\n",
    "\n",
    "$$\n",
    "P v^\\prime = \\mathit{0}\n",
    "$$\n",
    "\n",
    "Thus\n",
    "\n",
    "$$\n",
    "v^\\prime = v^\\prime - P v^\\prime\n",
    "$$\n",
    "\n",
    "And since $\\operatorname{Ker} P \\subseteq V$, thus $v^\\prime \\in V$.\n",
    "\n",
    "Thus $\\operatorname{Ker} P \\subseteq V^\\prime$.\n",
    "\n",
    "Hence $V^\\prime = \\operatorname{Ker} P$.\n",
    "\n",
    "#### Proof: $\\{v^{\\prime\\prime} \\in V | [\\exists v \\in V] v^{\\prime\\prime} = P v\\} = \\operatorname{Im} P$\n",
    "\n",
    "This is obvious.\n",
    "\n",
    "Thus for any element $v \\in V$ can be written as a sum of $v^\\prime + v^{\\prime\\prime}$ for $v^\\prime \\in \\operatorname{Ker} P$ and $v^{\\prime\\prime} \\in \\operatorname{Im} P$. \n",
    "\n",
    "Thus $V$ the direct sum of $\\operatorname{Ker} P$ and $\\operatorname{Im} P$ Q.E.D."
   ]
  },
  {
   "cell_type": "code",
   "execution_count": null,
   "metadata": {},
   "outputs": [],
   "source": []
  }
 ],
 "metadata": {
  "kernelspec": {
   "display_name": "Python 3",
   "language": "python",
   "name": "python3"
  },
  "language_info": {
   "codemirror_mode": {
    "name": "ipython",
    "version": 3
   },
   "file_extension": ".py",
   "mimetype": "text/x-python",
   "name": "python",
   "nbconvert_exporter": "python",
   "pygments_lexer": "ipython3",
   "version": "3.7.0"
  }
 },
 "nbformat": 4,
 "nbformat_minor": 2
}
